

Solutions to Probability Problems

Xiankang Wang

November 7, 2025

Contents

1	Problem 1: Event Probabilities	2
1.1	Problem Statement	2
1.2	Solution	2
2	Problem 2: Exponential Distribution Transformation	3
2.1	Problem Statement	3
2.2	Solution	3
3	Problem 3: Joint, Marginal, and Conditional Densities	4
3.1	Problem Statement	4
3.2	Solution	4
4	Problem 4: Functions of Exponential Variables	6
4.1	Problem Statement	6
4.2	Solution	6
5	Problem 5: Derived Discrete Variables	8
5.1	Problem Statement	8
5.2	Solution	8

1 Problem 1: Event Probabilities

1.1 Problem Statement

Let A, B denote two events. \bar{A} is the complement set of A , and \bar{B} is the complement set of B . Given that $P(A) = x$, $P(B) = y$, $P(A \cap B) = z$, please find the probability of the following using x, y, z :

(a) $P(\bar{A} \cap B)$.

(b) $P(\bar{A} \cap \bar{B})$.

(c) $P(\bar{A} \cup B)$.

(d) $P(\bar{A} \cup \bar{B})$.

1.2 Solution

(a) $P(\bar{A} \cap B)$. This is the probability that event B occurs but event A does not. We can find this by subtracting the probability of both events occurring from the probability of event B .

$$P(\bar{A} \cap B) = P(B) - P(A \cap B) = \boxed{y - z}.$$

(b) $P(\bar{A} \cap \bar{B})$. This is the probability that neither A nor B occurs. By De Morgan's laws, $\bar{A} \cap \bar{B} = \overline{A \cup B}$.

$$P(\bar{A} \cap \bar{B}) = P(\overline{A \cup B}) = 1 - P(A \cup B).$$

Using the principle of inclusion-exclusion for $P(A \cup B)$:

$$P(A \cup B) = P(A) + P(B) - P(A \cap B) = x + y - z.$$

Therefore,

$$P(\bar{A} \cap \bar{B}) = 1 - (x + y - z) = \boxed{1 - x - y + z}.$$

(c) $P(\bar{A} \cup B)$. Using the probability addition rule:

$$P(\bar{A} \cup B) = P(\bar{A}) + P(B) - P(\bar{A} \cap B).$$

We know $P(\bar{A}) = 1 - P(A) = 1 - x$, and from part (a), $P(\bar{A} \cap B) = y - z$. Substituting these in:

$$P(\bar{A} \cup B) = (1 - x) + y - (y - z) = \boxed{1 - x + z}.$$

(d) $P(\bar{A} \cup \bar{B})$. By De Morgan's laws, $\bar{A} \cup \bar{B} = \overline{A \cap B}$.

$$P(\bar{A} \cup \bar{B}) = P(\overline{A \cap B}) = 1 - P(A \cap B) = \boxed{1 - z}.$$

2 Problem 2: Exponential Distribution Transformation

2.1 Problem Statement

Let random variable X have an exponential distribution with $EX = 1$. Let $Y = X^2 - 2$.

- (a) Find the moment generating function of X .
- (b) Find the probability density function of Y .
- (c) Find the mean and the variance of Y .

2.2 Solution

For an exponential distribution with parameter λ , the PDF is $f(x) = \lambda e^{-\lambda x}$ and the expectation is $EX = 1/\lambda$. Given $EX = 1$, we have $1/\lambda = 1$, so $\lambda = 1$. Thus, X follows a standard exponential distribution with PDF $f_X(x) = e^{-x}$ for $x > 0$.

(a) Moment generating function (MGF) of X . The MGF is defined as $M_X(t) = E[e^{tX}]$.

$$M_X(t) = \int_0^\infty e^{tx} f_X(x) dx = \int_0^\infty e^{tx} e^{-x} dx = \int_0^\infty e^{(t-1)x} dx.$$

For the integral to converge, we require $t - 1 < 0$, or $t < 1$.

$$M_X(t) = \left[\frac{1}{t-1} e^{(t-1)x} \right]_0^\infty = 0 - \frac{1}{t-1} = \boxed{\frac{1}{1-t}}, \quad \text{for } t < 1.$$

(b) Probability density function (PDF) of Y . We first find the CDF of Y , $F_Y(y) = P(Y \leq y)$, for y in the support of Y . Since $X > 0$, $X^2 > 0$, so $Y = X^2 - 2 > -2$. For $y > -2$:

$$F_Y(y) = P(X^2 - 2 \leq y) = P(X^2 \leq y + 2).$$

Since X is always positive, this is equivalent to:

$$F_Y(y) = P(0 < X \leq \sqrt{y+2}) = F_X(\sqrt{y+2}).$$

The CDF of $X \sim \text{Exp}(1)$ is $F_X(x) = 1 - e^{-x}$ for $x > 0$. So,

$$F_Y(y) = 1 - e^{-\sqrt{y+2}}.$$

To find the PDF, we differentiate the CDF with respect to y :

$$f_Y(y) = \frac{d}{dy} F_Y(y) = \frac{d}{dy} (1 - e^{-\sqrt{y+2}}) = -e^{-\sqrt{y+2}} \cdot \left(-\frac{1}{2\sqrt{y+2}} \right).$$

$$f_Y(y) = \boxed{\frac{e^{-\sqrt{y+2}}}{2\sqrt{y+2}}}, \quad \text{for } y > -2.$$

(c) Mean and variance of Y . We use the properties of expectation and variance. For $X \sim \text{Exp}(1)$, the k -th moment is $E[X^k] = k!$. The mean of Y :

$$E[Y] = E[X^2 - 2] = E[X^2] - 2.$$

$$E[X^2] = 2! = 2.$$

$$E[Y] = 2 - 2 = \boxed{0}.$$

The variance of Y :

$$\text{Var}(Y) = \text{Var}(X^2 - 2) = \text{Var}(X^2) = E[(X^2)^2] - (E[X^2])^2 = E[X^4] - (E[X^2])^2.$$

$$E[X^4] = 4! = 24.$$

$$\text{Var}(Y) = 24 - (2)^2 = 24 - 4 = \boxed{20}.$$

3 Problem 3: Joint, Marginal, and Conditional Densities

3.1 Problem Statement

The joint probability density function of X and Y is given by

$$f_{XY}(x, y) = \begin{cases} c(x^2 - y^2)e^{-x}, & 0 < x < \infty, -x < y < x \\ 0, & \text{otherwise.} \end{cases}$$

- (a) What is the value of c ?
- (b) Find the marginal probability density function of X .
- (c) Find the EY .
- (d) Find the conditional density function of Y , given $X = x$.

3.2 Solution

(a) **Value of c .** The total probability must be 1.

$$\int_0^\infty \int_{-x}^x c(x^2 - y^2)e^{-x} dy dx = 1.$$

First, we solve the inner integral with respect to y :

$$\int_{-x}^x (x^2 - y^2) dy = \left[x^2 y - \frac{y^3}{3} \right]_{-x}^x = \left(x^3 - \frac{x^3}{3} \right) - \left(-x^3 + \frac{x^3}{3} \right) = \frac{2x^3}{3} - \left(-\frac{2x^3}{3} \right) = \frac{4x^3}{3}.$$

Now, we solve the outer integral:

$$c \int_0^\infty \frac{4x^3}{3} e^{-x} dx = 1 \implies \frac{4c}{3} \int_0^\infty x^3 e^{-x} dx = 1.$$

The integral is the Gamma function $\Gamma(4) = 3! = 6$.

$$\frac{4c}{3} \cdot 6 = 1 \implies 8c = 1 \implies \boxed{c = \frac{1}{8}}.$$

(b) **Marginal PDF of X .** We integrate the joint PDF over all possible values of y .

$$f_X(x) = \int_{-x}^x f_{XY}(x, y) dy = \int_{-x}^x \frac{1}{8}(x^2 - y^2)e^{-x} dy.$$

This is $\frac{1}{8}e^{-x}$ times the inner integral from part (a):

$$f_X(x) = \frac{1}{8}e^{-x} \left(\frac{4x^3}{3} \right) = \boxed{\frac{1}{6}x^3 e^{-x}}, \quad \text{for } x > 0.$$

(c) **Expectation of Y .**

$$E[Y] = \int_0^\infty \int_{-x}^x y f_{XY}(x, y) dy dx = \int_0^\infty \int_{-x}^x y \frac{1}{8}(x^2 - y^2)e^{-x} dy dx.$$

Consider the inner integral:

$$\int_{-x}^x y(x^2 - y^2) dy = \int_{-x}^x (x^2 y - y^3) dy.$$

The integrand $g(y) = x^2 y - y^3$ is an odd function of y , and it is integrated over a symmetric interval $[-x, x]$. Therefore, the integral is 0.

$$E[Y] = \int_0^\infty \frac{1}{8}e^{-x}(0) dx = \boxed{0}.$$

(d) Conditional PDF of Y given $X = x$. The conditional density is given by $f_{Y|X}(y|x) = \frac{f_{XY}(x,y)}{f_X(x)}$ for $f_X(x) > 0$.

$$f_{Y|X}(y|x) = \frac{\frac{1}{8}(x^2 - y^2)e^{-x}}{\frac{1}{6}x^3e^{-x}}.$$

The term e^{-x} cancels out. The domain for y is $-x < y < x$.

$$f_{Y|X}(y|x) = \frac{1/8}{1/6} \cdot \frac{x^2 - y^2}{x^3} = \frac{6}{8} \frac{x^2 - y^2}{x^3} = \boxed{\frac{3}{4x^3}(x^2 - y^2)}, \quad \text{for } -x < y < x.$$

4 Problem 4: Functions of Exponential Variables

4.1 Problem Statement

Let Z be an exponentially distributed random variable with mean β .

- (a) Find the probability density function of $X = -\ln \frac{Z}{\beta}$.
- (b) Suppose X_1 and X_2 are two independent random variables following the same distribution as X . Find the probability density function of $X_1 - X_2$.
- (c) Suppose X_1, X_2, \dots, X_n are independent random variables following the same distribution as X . Show that $\max(X_2, X_3, \dots, X_n)$ and $X_1 + \ln(n-1)$ are identically distributed.

4.2 Solution

The PDF of $Z \sim \text{Exp}(\text{mean} = \beta)$ is $f_Z(z) = \frac{1}{\beta}e^{-z/\beta}$ for $z > 0$. The CDF is $F_Z(z) = 1 - e^{-z/\beta}$.

(a) PDF of $X = -\ln(Z/\beta)$. We find the CDF of X first.

$$\begin{aligned} F_X(x) &= P(X \leq x) = P(-\ln(Z/\beta) \leq x) = P(\ln(Z/\beta) \geq -x) \\ &= P(Z/\beta \geq e^{-x}) = P(Z \geq \beta e^{-x}). \end{aligned}$$

This is $1 - F_Z(\beta e^{-x}) = 1 - (1 - e^{-(\beta e^{-x})/\beta}) = e^{-e^{-x}}$. So, the CDF is $F_X(x) = e^{-e^{-x}}$. The PDF is the derivative of the CDF:

$$f_X(x) = \frac{d}{dx} \left(e^{-e^{-x}} \right) = e^{-e^{-x}} \cdot (-e^{-x}) \cdot (-1) = \boxed{e^{-x} e^{-e^{-x}}}.$$

This is the standard Gumbel distribution.

(b) PDF of $Y = X_1 - X_2$. Let $U_i = Z_i/\beta \sim \text{Exp}(1)$. Then $X_i = -\ln U_i$. So, $Y = X_1 - X_2 = (-\ln U_1) - (-\ln U_2) = \ln(U_2/U_1)$. We find the CDF of Y : $F_Y(y) = P(Y \leq y) = P(\ln(U_2/U_1) \leq y) = P(U_2 \leq U_1 e^y)$. We integrate over the distribution of U_1 :

$$\begin{aligned} F_Y(y) &= \int_0^\infty P(U_2 \leq u_1 e^y) f_{U_1}(u_1) du_1 = \int_0^\infty (1 - e^{-u_1 e^y}) e^{-u_1} du_1 \\ &= \int_0^\infty (e^{-u_1} - e^{-(1+e^y)u_1}) du_1 = [-e^{-u_1}]_0^\infty - \left[-\frac{e^{-(1+e^y)u_1}}{1+e^y} \right]_0^\infty \\ &= (1) - \left(\frac{1}{1+e^y} \right) = \frac{e^y}{1+e^y} = \frac{1}{1+e^{-y}}. \end{aligned}$$

This is the CDF of the standard logistic distribution. Differentiating to find the PDF:

$$f_Y(y) = \frac{d}{dy} \left(\frac{e^y}{1+e^y} \right) = \frac{e^y(1+e^y) - e^y(e^y)}{(1+e^y)^2} = \boxed{\frac{e^y}{(1+e^y)^2}}.$$

(c) Show identical distribution. Let $V = X_1 + \ln(n-1)$ and $M = \max(X_2, \dots, X_n)$. We show they have the same CDF. First, the CDF of V :

$$\begin{aligned} F_V(v) &= P(V \leq v) = P(X_1 + \ln(n-1) \leq v) = P(X_1 \leq v - \ln(n-1)). \\ &= F_X(v - \ln(n-1)) = \exp(-\exp(-(v - \ln(n-1)))) = \exp(-\exp(-v + \ln(n-1))) \\ &= \exp(-e^{-v} \cdot e^{\ln(n-1)}) = \exp(-(n-1)e^{-v}). \end{aligned}$$

Next, the CDF of M :

$$F_M(m) = P(M \leq m) = P(\max(X_2, \dots, X_n) \leq m).$$

This is equivalent to $P(X_2 \leq m, X_3 \leq m, \dots, X_n \leq m)$. Due to independence and identical distribution:

$$\begin{aligned} F_M(m) &= P(X_2 \leq m) \cdots P(X_n \leq m) = [F_X(m)]^{n-1}. \\ &= (e^{-e^{-m}})^{n-1} = \exp(-(n-1)e^{-m}). \end{aligned}$$

Since $F_V(x) = F_M(x)$ for all x , the two random variables are identically distributed.

5 Problem 5: Derived Discrete Variables

5.1 Problem Statement

Suppose the probability density function of random variable Y is $f_Y(y) = e^{-y}$ for $y > 0$. Define the random variables X_i as follows:

$$X_i = \begin{cases} 1, & Y > i \\ 0, & Y \leq i \end{cases} \quad \text{for } i = 1, 2.$$

- (a) Let $Z = e^{X_1}$. Find the probability mass function of Z .
- (b) Find the joint probability mass function of (X_1, X_2) .

5.2 Solution

The given distribution for Y is standard exponential, $Y \sim \text{Exp}(1)$. We have $P(Y > y) = e^{-y}$ and $P(Y \leq y) = 1 - e^{-y}$.

(a) **PMF of $Z = e^{X_1}$.** First, we find the PMF of X_1 . X_1 can take values 0 or 1.

$$P(X_1 = 1) = P(Y > 1) = e^{-1}.$$

$$P(X_1 = 0) = P(Y \leq 1) = 1 - e^{-1}.$$

Now, we find the possible values of Z and their probabilities.

- If $X_1 = 0$, then $Z = e^0 = 1$. This occurs with probability $P(X_1 = 0) = 1 - e^{-1}$.
- If $X_1 = 1$, then $Z = e^1 = e$. This occurs with probability $P(X_1 = 1) = e^{-1}$.

So, the PMF of Z , denoted $p_Z(z)$, is:

$$p_Z(z) = \begin{cases} 1 - e^{-1}, & z = 1 \\ e^{-1}, & z = e \\ 0, & \text{otherwise.} \end{cases}$$

(b) **Joint PMF of (X_1, X_2) .** The vector (X_1, X_2) can take four possible values: $(0, 0)$, $(0, 1)$, $(1, 0)$, $(1, 1)$. We compute the probability for each case.

- $P(X_1 = 0, X_2 = 0) = P(Y \leq 1 \text{ and } Y \leq 2) = P(Y \leq 1) = \boxed{1 - e^{-1}}$.
- $P(X_1 = 0, X_2 = 1) = P(Y \leq 1 \text{ and } Y > 2)$. These are disjoint events, so the probability is $\boxed{0}$.
- $P(X_1 = 1, X_2 = 0) = P(Y > 1 \text{ and } Y \leq 2) = P(1 < Y \leq 2) = P(Y \leq 2) - P(Y \leq 1) = (1 - e^{-2}) - (1 - e^{-1}) = \boxed{e^{-1} - e^{-2}}$.
- $P(X_1 = 1, X_2 = 1) = P(Y > 1 \text{ and } Y > 2) = P(Y > 2) = \boxed{e^{-2}}$.

The joint PMF $p(x_1, x_2)$ can be summarized in a table:

$p(x_1, x_2)$	$X_2 = 0$	$X_2 = 1$
$X_1 = 0$	$1 - e^{-1}$	0
$X_1 = 1$	$e^{-1} - e^{-2}$	e^{-2}